LeanBoogie/ITree/QITree.lean
@@ -1,0 +1,91 @@
+import LeanBoogie.ITree.Eutt
+import Mathlib.Data.Quot
+
+/-
+  # Quotient of ITree along Eutt
+-/
+
+def QITree (E A : Type) : Type := Quotient (α := ITree E A) ITree.setoid
+def QITree.ret (a : A) : QITree E A := Quotient.mk ITree.setoid (ITree.ret a)
+def QITree.tau (t : QITree E A) : QITree E A := Quotient.liftOn t (⟦ITree.tau ·⟧) (by
+  intro t t' h
+  have : t.tau ≈ t'.tau := Eutt.tau_congr h
+  simp only [eq_rec_constant]
+  exact Quotient.sound this
+)
+
+opaque QITree.vis_impl (e : E) (k : Ans -> QITree E A) : QITree E A := sorry
+
+-- https://leanprover.zulipchat.com/#narrow/channel/113488-general/topic/Quot.20lifting.20.60.28_.20-.3E.20T.29.20-.3E.20T.60.20to.20.60.28_.20-.3E.20Q.29.20-.3E.20Q.60/near/484606314
+@[implemented_by QITree.vis_impl]
+def QITree.vis (e : E) (k : Ans -> QITree E A) : QITree E A :=
+  Quotient.liftOn (Quotient.choice k) (⟦ITree.vis e ·⟧) (fun _ _ => Quotient.eq.mpr ∘ Eutt.vis)
+
+#check Quot.lift
+#check Quotient.sound
+
+example (t : QITree E A) : QITree.tau t = t := by
+  simp [QITree.tau]
+  dsimp [Quotient.liftOn, Quot.liftOn, Quotient.mk]
+
+  sorry
+
+set_option pp.proofs true in
+def QITree.cases {E A : Type} {motive : QITree E A → Sort u}
+    (c_ret : (r : A) → motive (.ret r))
+    (c_tau : (x : QITree E A) → motive (.tau x))
+    (c_vis : (e : E) → (k : Ans → QITree E A) → motive (.vis e k))
+    (x : QITree E A)
+    : motive x
+    := Quotient.recOn x
+      (ITree.cases
+        c_ret
+        (fun t => c_tau ⟦t⟧)
+        (fun e k =>
+          have : (QITree.vis e fun ans => ⟦k ans⟧) = ⟦ITree.vis e k⟧ := by simp only [QITree.vis, Quotient.choice_eq, Quotient.lift_mk]
+          this ▸ c_vis e (fun ans => ⟦k ans⟧)))
+      (fun a b h => by
+        simp
+        cases a
+        case ret r =>-- provable
+          cases b
+          case ret r => sorry
+          case tau t => sorry
+          case vis e k => sorry
+        case tau t =>
+          cases b
+          case ret r =>
+            simp [ITree.cases_tau, ITree.cases_ret, ITree.cases_vis]
+            have h : t ≈ .ret r := sorry
+            -- We know that t converges to `.ret r`, and emits no events.
+            have := Quotient.sound h
+            -- We can obtain any proof `⟦.ret r⟧ = ⟦t⟧ = ⟦t.tau⟧ = ⟦t.tau.tau⟧ = ⟦t.tau.tau.tau⟧ = ...`
+            -- By function extensionality (sort of...?) we can know that `c_tau ⟦.ret r⟧ = c_tau ⟦t⟧ = c_tau ⟦t.tau⟧ = ...`
+
+            -- this is not provable... (or only provable if our motive is `... -> Prop`)
+            sorry
+          case tau t =>
+            simp [ITree.cases_tau, ITree.cases_ret, ITree.cases_vis]
+            sorry
+          case vis e k =>
+            simp [ITree.cases_tau, ITree.cases_ret, ITree.cases_vis]
+            sorry
+        case vis e k =>
+          cases b
+          case ret r => sorry
+          case tau t => sorry
+          case vis e k => sorry
+      )
+
+set_option pp.proofs true in
+def QITree.cases_2 {E A : Type} {motive : QITree E A → Sort u}
+  (c_ret : (r : A) → motive (.ret r))
+  -- (tau : (x : QITree E A) → motive (.tau x)) -- // Note: Even with quotients we can't get rid of this case. Imagine `QITree.cases (motive := False when .tau) c_ret c_vis spin : False`. Or... maybe this is okay, because we can not write that motive type in the first place, since we can't distinguish between `.ret : QITree` and `.tau _ : QITree`.
+  (c_vis : (e : E) → (k : Ans → QITree E A) → motive (.vis e k))
+  (x : QITree E A)
+  : motive x
+  := Quotient.liftOn₂ (Quotient.choice)
+
+
+
+-- TODO: QITree.corec... which has a lot of references to `Shape` and `Base` :(
